tools/poly/Listsort.sig
@@ -1,0 +1,17 @@
+(* Listsort *)
+signature Listsort =
+sig
+
+val sort   : ('a * 'a -> order) -> 'a list -> 'a list
+val sorted : ('a * 'a -> order) -> 'a list -> bool
+
+end;
+
+(*
+   [sort ordr xs] sorts the list xs in nondecreasing order, using the
+   given ordering.  Uses Richard O'Keefe's smooth applicative merge
+   sort.
+
+   [sorted ordr xs] checks that the list xs is sorted in nondecreasing
+   order, in the given ordering.
+*)
