tools/poly/Listsort.sml
@@ -1,0 +1,41 @@
+structure Listsort :> Listsort =
+struct
+(* Listsort *)
+
+(** Smooth Applicative Merge Sort, Richard O'Keefe 1982        **)
+(** From L.C. Paulson: ML for the Working Programmer, CUP 1991 **)
+(** Optimized for Moscow ML **)
+
+fun sort ordr []          = []
+  | sort ordr (xs as [_]) = xs
+  | sort ordr (xs as [x1, x2]) =
+    (case ordr(x1, x2) of
+	 GREATER => [x2, x1]
+       | _       => xs)
+  | sort ordr xs =
+    let fun merge []      ys = ys
+          | merge xs      [] = xs
+          | merge (x::xs) (y::ys) =
+            if ordr(x, y) <> GREATER then x :: merge xs (y::ys)
+            else y :: merge (x::xs) ys
+        fun mergepairs l1  []              k = [l1]
+          | mergepairs l1 (ls as (l2::lr)) k =
+            if k mod 2 = 1 then l1::ls
+            else mergepairs (merge l1 l2) lr (k div 2)
+	fun nextrun run []      = (run, [])
+	  | nextrun run (xs as (x::xr)) =
+	    if ordr(x, List.hd run) = LESS then (run, xs)
+	    else nextrun (x::run) xr
+        fun sorting []      ls r = List.hd(mergepairs [] ls 0)
+          | sorting (x::xs) ls r =
+	    let val (revrun, tail) = nextrun [x] xs
+	    in sorting tail (mergepairs (List.rev revrun) ls (r+1)) (r+1) end
+    in sorting xs [] 0 end;
+
+fun sorted ordr []         = true
+  | sorted ordr (y1 :: yr) =
+    let fun h x0 []       = true
+	  | h x0 (x1::xr) = ordr(x0, x1) <> GREATER andalso h x1 xr
+    in h y1 yr end;
+
+end;
