tools/poly/Portable.sml
@@ -1,0 +1,216 @@
+(* ===================================================================== *)
+(* FILE          : Portable.sml                                          *)
+(* DESCRIPTION   : Structure for SML System dependent functions.         *)
+(* AUTHOR        : Ken Larsen, University of Cambridge (or DTU)          *)
+(*                 based on code by                                      *)
+(*                 Elsa L. Gunter, AT&T Bell Laboratories                *)
+(* DATE          : 19 September, 1997                                    *)
+(* ===================================================================== *)
+
+(* Copyright 1993 by AT&T Bell Laboratories *)
+(* Copyright 1997 by University of Cambridge *)
+
+(* Share and Enjoy *)
+
+structure Portable :> Portable =
+struct
+
+exception Div = General.Div
+exception Mod = General.Div
+exception Interrupt = SML90.Interrupt
+
+(*---------------------------------------------------------------------------
+      Refs
+ ---------------------------------------------------------------------------*)
+
+fun inc r = (r := !r + 1)
+fun dec r = (r := !r - 1);
+
+
+(*---------------------------------------------------------------------------
+   SML/NJ v.93 style string operations
+ ---------------------------------------------------------------------------*)
+
+fun ordof (string,place) = Char.ord(String.sub(string,place))
+val implode = String.concat;
+val explode = map Char.toString o String.explode;
+
+(*---------------------------------------------------------------------------
+    System
+ ---------------------------------------------------------------------------*)
+
+structure Process = OS.Process
+structure FileSys = OS.FileSys
+val getEnv   = Process.getEnv
+val cd       = FileSys.chDir
+val pwd      = FileSys.getDir
+fun listDir s = let
+  val ds = FileSys.openDir s
+  fun recurse acc =
+      case FileSys.readDir ds of
+        NONE => acc
+      | SOME f => recurse (f :: acc)
+in
+  recurse [] before FileSys.closeDir ds
+end
+
+fun system s = if Process.isSuccess (Process.system s) then 0 else 1
+val getArgs  = CommandLine.arguments
+val argv     = getArgs
+fun exit()   = Process.exit Process.success
+
+
+(*---------------------------------------------------------------------------
+    IO
+ ---------------------------------------------------------------------------*)
+
+exception Io of string;
+type instream      = TextIO.instream
+type outstream     = TextIO.outstream
+val std_out        = TextIO.stdOut
+val stdin          = TextIO.stdIn
+fun open_in file   = TextIO.openIn file
+                     handle IO.Io{cause=OS.SysErr(s,_),...} => raise (Io s)
+                                   (* handle OS.SysErr (s,_) => raise Io s; *)
+fun open_out file  = TextIO.openOut file
+                     handle IO.Io{cause=OS.SysErr(s,_),...} => raise (Io s)
+                                   (* handle OS.SysErr (s,_) => raise Io s; *)
+val output         = TextIO.output
+fun outputc strm s = output(strm,s)
+val close_in       = TextIO.closeIn
+val close_out      = TextIO.closeOut
+val flush_out      = TextIO.flushOut
+fun input_line strm =
+  case TextIO.inputLine strm of
+    NONE => ""
+  | SOME s => s
+val end_of_stream  = TextIO.endOfStream
+
+(*---------------------------------------------------------------------------
+    Efficiency hack.
+ ---------------------------------------------------------------------------*)
+
+fun pointer_eq (x:'a, y:'a) = PolyML.pointerEq(x,y)
+
+(*---------------------------------------------------------------------------
+    Time
+ ---------------------------------------------------------------------------*)
+
+type time = Time.time
+
+local open Time
+in
+  val timestamp : unit -> time = now
+  val time_to_string : time -> string = toString
+  fun dest_time t =
+     let val r = toReal t
+         val sec = Arbnum.floor (toReal t)
+         val sec_million = Arbnum.*(sec, Arbnum.fromInt 1000000)
+         val r_million = r * 1000000.0
+         val usec = Arbnum.-(Arbnum.floor r_million, sec_million)
+     in
+        {sec=sec, usec=usec}
+     end
+  fun mk_time {sec,usec} =
+      fromReal (Real.+(Arbnum.toReal sec, Arbnum.toReal usec / 1000000.0))
+  fun time_eq (t1:time) t2 = (t1 = t2)
+  fun time_lt (t1:time) t2 = Time.<(t1,t2)
+end
+
+
+(*---------------------------------------------------------------------------
+    Pretty Printing
+ ---------------------------------------------------------------------------*)
+
+open PP
+
+type ppstream = General.ppstream;
+
+fun with_ppstream ppstrm =
+  {add_string     = add_string ppstrm,
+   add_break      = add_break ppstrm,
+   begin_block    = begin_block ppstrm,
+   end_block      = fn () => end_block ppstrm,
+   add_newline    = fn () => add_newline ppstrm,
+   clear_ppstream = fn () => clear_ppstream ppstrm,
+   flush_ppstream = fn () => flush_ppstream ppstrm}
+
+fun defaultConsumer () =
+   {consumer  = fn s => TextIO.output(TextIO.stdOut, s),
+    linewidth = 72,
+    flush     = fn () => TextIO.flushOut TextIO.stdOut}
+
+fun pp_to_string linewidth ppfn ob =
+    let val l = ref ([]:string list)
+	fun attach s = l := (s::(!l))
+    in with_pp {consumer = attach,
+		linewidth=linewidth, flush = fn()=>()}
+               (fn ppstrm =>  ppfn ppstrm ob);
+	String.concat(List.rev(!l))
+    end
+
+val mk_consumer = fn x => x
+
+(*---------------------------------------------------------------------------*)
+(* Generate a standard ppstream                                              *)
+(*---------------------------------------------------------------------------*)
+
+fun stdOut_ppstream () = mk_ppstream (defaultConsumer());
+
+(*---------------------------------------------------------------------------
+ * Print a list of items.
+ *
+ *     pfun = print_function
+ *     dfun = delim_function
+ *     bfun = break_function
+ *---------------------------------------------------------------------------*)
+
+fun pr_list_to_ppstream ppstrm pfun dfun bfun =
+ let fun pr [] = ()
+       | pr [i] = pfun ppstrm i
+       | pr (i::rst) = ( pfun ppstrm i; dfun ppstrm ; bfun ppstrm ; pr rst )
+ in pr end;
+
+
+(*---------------------------------------------------------------------------
+ * Simple and heavily used.
+ * pfun = item printing function
+ * dfun = delimiter printing function
+ * bfun = break printer function
+ *---------------------------------------------------------------------------*)
+
+fun pr_list pfun dfun bfun =
+   let fun pr [] = ()
+         | pr [i] = pfun i
+         | pr (i::rst) = ( pfun i; dfun() ; bfun() ; pr rst )
+   in pr end;
+
+(*---------------------------------------------------------------------------*)
+(* Send the results of prettyprinting to stdOut                              *)
+(*---------------------------------------------------------------------------*)
+
+fun pprint pp x =
+ let val strm = stdOut_ppstream ()
+ in
+   let val _  = pp strm x
+   in flush_ppstream strm; ()
+   end handle e => (flush_ppstream strm; raise e)
+ end;
+
+
+
+datatype 'a frag = QUOTE of string | ANTIQUOTE of 'a
+type 'a quotation = 'a frag list;
+
+(*---------------------------------------------------------------------------
+      MoscowML returns lists of QUOTE'd strings when a quote is spread
+      over more than one line. "norm_quote" concatenates all adjacent
+      QUOTE elements in this list.
+ ---------------------------------------------------------------------------*)
+
+fun norm_quote [] = []
+  | norm_quote [x] = [x]
+  | norm_quote (QUOTE s1::QUOTE s2::rst) = norm_quote (QUOTE(s1^s2)::rst)
+  | norm_quote (h::rst) = h::norm_quote rst;
+
+end (* Portable *)
