examples/euclid.sml
@@ -5,30 +5,32 @@
 (*                                                                           *)
 (*===========================================================================*)
 
-(*---------------------------------------------------------------------------*
- * First, open some relevant support.                                        *
- *---------------------------------------------------------------------------*)
+(*---------------------------------------------------------------------------*)
+(* First, open some relevant context, the theory of arithmetic. This theory  *)
+(* is already present, but the ML module arithmeticTheory needs to be opened *)
+(* before the definitions and theorems of the theory are available without   *)
+(* supplying the "arithmeticTheory." prefix.
+(*---------------------------------------------------------------------------*)
 
 open arithmeticTheory
-
-val ARW_TAC = RW_TAC arith_ss;
-
 
 (*---------------------------------------------------------------------------*)
 (* Divisibility.                                                             *)
 (*---------------------------------------------------------------------------*)
 
+val divides_def = 
+ Define 
+  `divides a b = ?x. b = a * x`;
+
 set_fixity "divides" (Infixr 450);
-
-val divides = Define `a divides b = ?x. b = a * x`;
-
 
 (*---------------------------------------------------------------------------*)
 (* Primality.                                                                *)
 (*---------------------------------------------------------------------------*)
 
-val prime = Define `prime p = ~(p=1) /\ !x. x divides p ==> (x=1) \/ (x=p)`;
-
+val prime_def = 
+ Define 
+   `prime p = ~(p=1) /\ !x. x divides p ==> (x=1) \/ (x=p)`;
 
 (*---------------------------------------------------------------------------*)
 (* A sequence of basic theorems about the "divides" relation.                *)
@@ -37,83 +39,102 @@ val prime = Define `prime p = ~(p=1) /\ !x. x divides p ==> (x=1) \/ (x=p)`;
 val DIVIDES_0 = store_thm
  ("DIVIDES_0",
   ``!x. x divides 0``,
-  PROVE_TAC [divides,MULT_CLAUSES]);
+  METIS_TAC [divides_def,MULT_CLAUSES]);
 
 val DIVIDES_ZERO = store_thm
  ("DIVIDES_ZERO",
   ``!x. 0 divides x = (x = 0)``,
-  PROVE_TAC [divides,MULT_CLAUSES]);
+  METIS_TAC [divides_def,MULT_CLAUSES]);
 
 val DIVIDES_ONE = store_thm
  ("DIVIDES_ONE",
   ``!x. x divides 1 = (x = 1)``,
-  PROVE_TAC [divides,MULT_CLAUSES,MULT_EQ_1]);
+  METIS_TAC [divides_def,MULT_CLAUSES,MULT_EQ_1]);
 
 val DIVIDES_REFL = store_thm
  ("DIVIDES_REFL",
   ``!x. x divides x``,
-  PROVE_TAC [divides,MULT_CLAUSES]);
+  METIS_TAC [divides_def,MULT_CLAUSES]);
 
 val DIVIDES_TRANS = store_thm
  ("DIVIDES_TRANS",
   ``!a b c. a divides b /\ b divides c ==> a divides c``,
-  PROVE_TAC [divides,MULT_ASSOC]);
+  METIS_TAC [divides_def,MULT_ASSOC]);
 
 val DIVIDES_ADD = store_thm
 ("DIVIDES_ADD",
  ``!d a b. d divides a /\ d divides b ==> d divides (a + b)``,
- PROVE_TAC[divides,LEFT_ADD_DISTRIB]);
+ METIS_TAC[divides_def,LEFT_ADD_DISTRIB]);
 
 val DIVIDES_SUB = store_thm
  ("DIVIDES_SUB",
   ``!d a b. d divides a /\ d divides b ==> d divides (a - b)``,
-  PROVE_TAC [divides,LEFT_SUB_DISTRIB]);
+  METIS_TAC [divides_def,LEFT_SUB_DISTRIB]);
 
 val DIVIDES_ADDL = store_thm
  ("DIVIDES_ADDL",
   ``!d a b. d divides a /\ d divides (a + b) ==> d divides b``,
-  PROVE_TAC [ADD_SUB,ADD_SYM,DIVIDES_SUB]);
+  METIS_TAC [ADD_SUB,ADD_SYM,DIVIDES_SUB]);
 
 val DIVIDES_LMUL = store_thm
  ("DIVIDES_LMUL",
   ``!d a x. d divides a ==> d divides (x * a)``,
-  PROVE_TAC [divides,MULT_ASSOC,MULT_SYM]);
+  METIS_TAC [divides_def,MULT_ASSOC,MULT_SYM]);
 
 val DIVIDES_RMUL = store_thm
  ("DIVIDES_RMUL",
   ``!d a x. d divides a ==> d divides (a * x)``,
-  PROVE_TAC [MULT_SYM,DIVIDES_LMUL]);
+  METIS_TAC [MULT_SYM,DIVIDES_LMUL]);
 
 val DIVIDES_LE = store_thm
  ("DIVIDES_LE",
   ``!m n. m divides n ==> m <= n \/ (n = 0)``,
-  ARW_TAC [divides]
+  RW_TAC arith_ss  [divides_def]
      THEN Cases_on `x`
-     THEN ARW_TAC [MULT_CLAUSES]);
+     THEN RW_TAC arith_ss  [MULT_CLAUSES]);
+
+(*---------------------------------------------------------------------------*)
+(* Various proofs of the same formula                                        *)
+(*---------------------------------------------------------------------------*)
 
 val DIVIDES_FACT = store_thm
  ("DIVIDES_FACT",
   ``!m n. 0 < m /\ m <= n ==> m divides (FACT n)``,
-  ARW_TAC [LESS_EQ_EXISTS]
+  RW_TAC arith_ss  [LESS_EQ_EXISTS]
    THEN Induct_on `p`
-   THEN ARW_TAC [FACT,ADD_CLAUSES]
+   THEN RW_TAC arith_ss  [FACT,ADD_CLAUSES]
    THENL [Cases_on `m`, ALL_TAC]
-   THEN PROVE_TAC [FACT, DECIDE ``!x. ~(x < x)``,
+   THEN METIS_TAC [FACT, DECIDE ``!x. ~(x < x)``,
                    DIVIDES_RMUL, DIVIDES_LMUL, DIVIDES_REFL]);
 
-(* Alternative proof *)
+val DIVIDES_FACT = store_thm
+ ("DIVIDES_FACT",
+  ``!m n. 0 < m /\ m <= n ==> m divides (FACT n)``,
+  RW_TAC arith_ss  [LESS_EQ_EXISTS]
+   THEN Induct_on `p`
+   THEN RW_TAC arith_ss  [FACT,ADD_CLAUSES]
+   THEN METIS_TAC [FACT, DECIDE ``!x. ~(x < x)``, num_CASES,
+                    DIVIDES_RMUL, DIVIDES_LMUL, DIVIDES_REFL]);
+
+val DIVIDES_FACT = store_thm
+ ("DIVIDES_FACT",
+  ``!m n. 0 < m /\ m <= n ==> m divides (FACT n)``,
+  RW_TAC arith_ss  [LESS_EQ_EXISTS]
+   THEN Induct_on `p`
+   THEN METIS_TAC [FACT, DECIDE ``!x. ~(x < x)``, num_CASES,
+                   DIVIDES_RMUL,DIVIDES_LMUL,DIVIDES_REFL,ADD_CLAUSES]);
+
+
 val DIVIDES_FACT = prove
 (``!m n. 0 < m /\ m <= n ==> m divides (FACT n)``,
 Induct_on `n - m`
- THEN ARW_TAC [] THENL
+ THEN RW_TAC arith_ss  [] THENL
  [`m = n`         by DECIDE_TAC THEN
-  `?k. m = SUC k` by PROVE_TAC[arithmeticTheory.num_CASES,
-                               prim_recTheory.LESS_REFL]
-     THEN PROVE_TAC[FACT,DIVIDES_RMUL,DIVIDES_REFL],
+  `?k. m = SUC k` by METIS_TAC[num_CASES,prim_recTheory.LESS_REFL]
+     THEN METIS_TAC[FACT,DIVIDES_RMUL,DIVIDES_REFL],
   `0 < n`         by DECIDE_TAC THEN
-  `?k. n = SUC k` by PROVE_TAC [arithmeticTheory.num_CASES,
-                                prim_recTheory.LESS_REFL]
-   THEN ARW_TAC [FACT, DIVIDES_RMUL]]);
+  `?k. n = SUC k` by METIS_TAC [num_CASES,prim_recTheory.LESS_REFL]
+   THEN RW_TAC arith_ss  [FACT, DIVIDES_RMUL]]);
 
 
 (*---------------------------------------------------------------------------*)
@@ -123,87 +144,99 @@ Induct_on `n - m`
 val NOT_PRIME_0 = store_thm
  ("NOT_PRIME_0",
   ``~prime 0``,
-  ARW_TAC [prime,DIVIDES_0]);
+  RW_TAC arith_ss  [prime_def,DIVIDES_0]);
 
 val NOT_PRIME_1 = store_thm
  ("NOT_PRIME_1",
   ``~prime 1``,
-  ARW_TAC [prime]);
+  RW_TAC arith_ss  [prime_def]);
 
 val PRIME_2 = store_thm
  ("PRIME_2",
   ``prime 2``,
-  ARW_TAC [prime] THEN
-  PROVE_TAC [DIVIDES_LE, DIVIDES_ZERO,
-             DECIDE``~(2=1) /\ ~(2=0) /\ (x <= 2 = (x=0) \/ (x=1) \/ (x=2))``]);
+  RW_TAC arith_ss  [prime_def] THEN
+  METIS_TAC [DIVIDES_LE, DIVIDES_ZERO,
+             DECIDE``~(2=1) /\ ~(2=0) /\ (x<=2 = (x=0) \/ (x=1) \/ (x=2))``]);
 
 val PRIME_POS = store_thm
  ("PRIME_POS",
   ``!p. prime p ==> 0<p``,
-  Cases THEN ARW_TAC[NOT_PRIME_0]);
+  Cases THEN RW_TAC arith_ss [NOT_PRIME_0]);
 
-(*---------------------------------------------------------------------------*
- * Every number has a prime factor, except for 1. The proof proceeds by a    *
- * "complete" induction on "n", and then considers cases on whether n is     *
- * prime or not. The first case (n is prime) is trivial. In the second case, *
- * there must be an "x" that divides n, and x is not 1 or n. By DIVIDES_LE,  *
- * n=0 or x <= n. If n=0, then 2 is a prime that divides 0. On the other     *
- * hand, if x <= n, there are two cases: if x<n then we can use the i.h. and *
- * by transitivity of divides we are done; otherwise, if x=n, then we have   *
- * a contradiction with the fact that x is not 1 or n.                       *
+(*---------------------------------------------------------------------------*)
+(* Every number has a prime factor, except for 1. The proof proceeds by a    *)
+(* "complete" induction on n, and then considers cases on whether n is       *)
+(* prime or not. The first case (n is prime) is trivial. In the second case, *)
+(* there must be an "x" that divides n, and x is not 1 or n. By DIVIDES_LE,  *)
+(* n=0 or x <= n. If n=0, then 2 is a prime that divides 0. On the other     *)
+(* hand, if x <= n, there are two cases: if x<n then we can use the i.h. and *)
+(* by transitivity of divides we are done; otherwise, if x=n, then we have   *)
+(* a contradiction with the fact that x is not 1 or n.                       *)
  *---------------------------------------------------------------------------*)
 
 val PRIME_FACTOR = store_thm
  ("PRIME_FACTOR",
   ``!n. ~(n = 1) ==> ?p. prime p /\ p divides n``,
   completeInduct_on `n`
-   THEN ARW_TAC []
+   THEN RW_TAC arith_ss  []
    THEN Cases_on `prime n` THENL
-   [PROVE_TAC [DIVIDES_REFL],
-    `?x. x divides n /\ ~(x=1) /\ ~(x=n)` by PROVE_TAC[prime]
-      THEN PROVE_TAC [LESS_OR_EQ, PRIME_2,
-                      DIVIDES_LE, DIVIDES_TRANS, DIVIDES_0]]);
+   [METIS_TAC [DIVIDES_REFL],
+    `?x. x divides n /\ ~(x=1) /\ ~(x=n)` by METIS_TAC[prime_def] THEN 
+    METIS_TAC [LESS_OR_EQ, PRIME_2,
+               DIVIDES_LE, DIVIDES_TRANS, DIVIDES_0]]);
+
+(*---------------------------------------------------------------------------*)
+(* In the following proof, METIS_TAC automatically considers cases on        *)
+(* whether n is prime or not.                                                *)
+(*---------------------------------------------------------------------------*)
+
+val PRIME_FACTOR = store_thm
+ ("PRIME_FACTOR",
+  ``!n. ~(n = 1) ==> ?p. prime p /\ p divides n``,
+  completeInduct_on `n` THEN 
+  METIS_TAC [DIVIDES_REFL,prime_def,LESS_OR_EQ, PRIME_2,
+             DIVIDES_LE, DIVIDES_TRANS, DIVIDES_0]);
 
 
-(*---------------------------------------------------------------------------*
- * Every number has a prime greater than it.                                 *
- * Proof.                                                                    *
- * Suppose not; then there's an "n" such that all "p" greater than n are     *
- * not prime. Consider FACT(n) + 1: it's not equal to 1, so there's a        *
- * prime p that divides it. p also divides FACT n because p is               *
- * less-than-or-equal to n. By DIVIDES_ADDL, this means that p=1. But        *
- * then p is not prime, which is a contradiction.                            *
- *---------------------------------------------------------------------------*)
+(*---------------------------------------------------------------------------*)
+(* Every number has a prime greater than it.                                 *)
+(* Proof.                                                                    *)
+(* Suppose not; then there's an n such that all p greater than n are not     *)
+(* prime. Consider FACT(n) + 1: it's not equal to 1, so there's a prime q    *)
+(* that divides it. q also divides FACT n because q is less-than-or-equal    *)
+(* to n. By DIVIDES_ADDL, this means that q=1. But then q is not prime,      *)
+(* which is a contradiction.                                                 *)
+(*---------------------------------------------------------------------------*)
 
 val EUCLID = store_thm
  ("EUCLID",
   ``!n. ?p. n < p /\ prime p``,
   SPOSE_NOT_THEN STRIP_ASSUME_TAC
    THEN MP_TAC (SPEC ``FACT n + 1`` PRIME_FACTOR)
-   THEN ARW_TAC [FACT_LESS, DECIDE ``~(x=0) = 0<x``]
-   THEN PROVE_TAC [DIVIDES_FACT, DIVIDES_ADDL, DIVIDES_ONE,
+   THEN RW_TAC arith_ss  [FACT_LESS, DECIDE ``~(x=0) = 0<x``]
+   THEN METIS_TAC [DIVIDES_FACT, DIVIDES_ADDL, DIVIDES_ONE,
                    NOT_PRIME_1, NOT_LESS, PRIME_POS]);
 
 
-(*---------------------------------------------------------------------------*
- * The previous proof is somewhat unsatisfactory, because its structure gets *
- * hidden in the invocations of the automated reasoners. An assertional      *
- * style allows a presentation that mirrors the informal proof.              *
- *---------------------------------------------------------------------------*)
+(*---------------------------------------------------------------------------*)
+(* The previous proof is somewhat unsatisfactory, because its structure gets *)
+(* hidden in the invocations of the automated reasoners. An assertional      *)
+(* style allows a presentation that mirrors the informal proof.              *)
+(*---------------------------------------------------------------------------*)
 
 val EUCLID_AGAIN = prove (``!n. ?p. n < p /\ prime p``,
 CCONTR_TAC
 THEN
-   `?n. !p. n < p ==> ~prime p`  by PROVE_TAC[]              THEN
-   `~(FACT n + 1 = 1)`           by ARW_TAC [FACT_LESS,
+   `?n. !p. n < p ==> ~prime p`  by METIS_TAC[]              THEN
+   `~(FACT n + 1 = 1)`           by RW_TAC arith_ss [FACT_LESS,
                                     DECIDE ``~(x=0) = 0<x``] THEN
    `?p. prime p /\
-        p divides (FACT n + 1)`  by PROVE_TAC [PRIME_FACTOR] THEN
-   `0 < p`                       by PROVE_TAC [PRIME_POS]    THEN
-   `p <= n`                      by PROVE_TAC [NOT_LESS]     THEN
-   `p divides FACT n`            by PROVE_TAC [DIVIDES_FACT] THEN
-   `p divides 1`                 by PROVE_TAC [DIVIDES_ADDL] THEN
-   `p = 1`                       by PROVE_TAC [DIVIDES_ONE]  THEN
-   `~prime p`                    by PROVE_TAC [NOT_PRIME_1]
+        p divides (FACT n + 1)`  by METIS_TAC [PRIME_FACTOR] THEN
+   `0 < p`                       by METIS_TAC [PRIME_POS]    THEN
+   `p <= n`                      by METIS_TAC [NOT_LESS]     THEN
+   `p divides FACT n`            by METIS_TAC [DIVIDES_FACT] THEN
+   `p divides 1`                 by METIS_TAC [DIVIDES_ADDL] THEN
+   `p = 1`                       by METIS_TAC [DIVIDES_ONE]  THEN
+   `~prime p`                    by METIS_TAC [NOT_PRIME_1]
 THEN
-PROVE_TAC[]);
+METIS_TAC[]);
